% !TeX encoding = UTF-8
% !TeX program = lualatex
% !TeX spellcheck = en_US

% Author : Zhihan Li
% Description : Report for Lecture 4 --- Best Approximation

\documentclass[english, nochinese]{../TeXTemplate/pkupaper}

\usepackage[paper, cmrgreekup]{../TeXTemplate/def}

\newcommand{\cuniversity}{Peking University}
\newcommand{\cthesisname}{Introduction to Applied Mathematics}
\newcommand{\titlemark}{Assignment for Lecture 4}

\DeclareRobustCommand{\authoring}%
{%
\begin{tabular}{c}%
Zhihan Li \\%
1600010653%
\end{tabular}%
}

\title{\titlemark}
\author{\authoring}
\begin{document}

\maketitle

\begin{thmquestion}
\
\begin{thmproof}
Prove by contradiction. Otherwise, there exists $ c = \msbr{ c_1 & c_2 & \cdots & c_m }^{\rmut} $, such that $ A c = 0 $, and therefore $ c^{\dag} A c = 0 $.

Note that
\begin{equation}
\begin{split}
c^{\dag} A c &= \sume{i}{1}{m}{\sume{j}{1}{m}{ \overline{c_j} \pbr{ g_j, g_i } c_i }} \\
&= \pbr{ \sume{j}{1}{m}{ \overline{c_j} g_j }, \sume{i}{1}{m}{ \overline{c_i} g_i } },
\end{split}
\end{equation}
and consequently from the positively definiteness
\begin{equation}
\sume{i}{1}{m}{ \overline{c_i} g_i } = 0.
\end{equation}
However this contradicts the given linear independence, which shows $A$ is non-singular.

\sqed
\end{thmproof}
\end{thmquestion}

\begin{thmquestion}
\ 
\begin{thmanswer}
Let the best approximation be $ g = \alpha x + \beta x^3 + \gamma x^5 $. From
\begin{equation}
f - g \perp \opspan \cbr{ x, x^3, x^5 },
\end{equation}
it can be derived that
\begin{gather}
\pbr{ f - g, x } = \pbr{ f - g, x^3 } = \pbr{ f - g, x^5 } = 0.
\end{gather}
Direct computation leads to the system
\begin{equation}
\left[\begin{matrix}\frac{2}{3} & \frac{2}{5} & \frac{2}{7}\\\frac{2}{5} & \frac{2}{7} & \frac{2}{9}\\\frac{2}{7} & \frac{2}{9} & \frac{2}{11}\end{matrix}\right] \msbr{ \alpha \\ \beta \\ \gamma } = \left[\begin{matrix}- 2 \cos{\left (1 \right )} + 2 \sin{\left (1 \right )}\\- 6 \sin{\left (1 \right )} + 10 \cos{\left (1 \right )}\\- 202 \cos{\left (1 \right )} + 130 \sin{\left (1 \right )}\end{matrix}\right],
\end{equation}
whose solution is
\begin{equation}
\msbr{ \alpha \\ \beta \\ \gamma } = \left[\begin{matrix}- \frac{139965}{8} \cos{\left (1 \right )} + 11235 \sin{\left (1 \right )}\\- \frac{104265}{2} \sin{\left (1 \right )} + \frac{324765}{4} \cos{\left (1 \right )}\\- \frac{582813}{8} \cos{\left (1 \right )} + \frac{93555}{2} \sin{\left (1 \right )}\end{matrix}\right].
\end{equation}
Therefore, the final solution is
\begin{equation}
\begin{split}
g &= x^{5} \left(- \frac{582813}{8} \cos{\left (1 \right )} + \frac{93555}{2} \sin{\left (1 \right )}\right) \\
&+ x^{3} \left(- \frac{104265}{2} \sin{\left (1 \right )} + \frac{324765}{4} \cos{\left (1 \right )}\right) \\
&+ x \left(- \frac{139965}{8} \cos{\left (1 \right )} + 11235 \sin{\left (1 \right )}\right).
\end{split}
\end{equation}
\end{thmanswer}
\end{thmquestion}

\begin{thmquestion}
\
\begin{thmproof}
Because
\begin{equation}
\norm{u_i} = \frac{\norm{ v_i - \sume{j}{1}{ i - 1 }{ \pbr{ v_i, u_j } u_j } }}{\norm{ v_i - \sume{j}{1}{ i - 1 }{ \pbr{ v_i, u_j } u_j } }} = 1
\end{equation}
for $ 1 \le i \le n $, it remains to prove $u_i$ are pairwise perpendicular.

Perform mathematical induction to prove that for a given $i$ with $ 1 \le i \le n $, $ u_j \perp u_k $ is always true for $ 1 \le j < k \le i $. Suppose the case $ i = m - 1  $ is done and then consider the case $ i = m $, where $ 1 < m \le n $. It is sufficient to prove $ u_m \perp u_k $ for $ 1 \le k < m $, which directly follows from
\begin{equation}
\pbr{ u_m, u_k } = \pbr{ v_m, u_k  } - \sume{j}{1}{ m - 1 }{ \pbr{ v_m, u_j } \pbr{ u_j, u_k } } = \pbr{ v_m, u_k } - \pbr{ v_m, u_k } \norm{u_k} = 0.
\end{equation}
Therefore, the induction is finished and we obtain $ u_j \perp u_k $ for $ 1 \le j < k \le n $.

As shown above, $u_i$ are pairwise orthogonal and normalized, which means they form a orthonormal basis.

\sqed
\end{thmproof}
\end{thmquestion}

\begin{thmquestion}
\
\begin{thmproof}
The leading coefficient of $L_n$ is
\begin{equation}
\frac{ \rbr{ 2 n } ! }{ 2^n n ! n ! } = \frac{ \rbr{ 2 n - 1 } !! }{ n ! },
\end{equation}
and therefore
\begin{equation}
g = \frac{ n ! }{ \rbr{ 2 n - 1 } !! } L_n
\end{equation}
is monic. Note that $ L_0, L_1, \cdots, L_{ n - 1 } $ form a basis of $ \opspan \cbr{ 1, x, \cdots, x^{ n - 1 } } $. Therefore, for any monic polynomial $f$ of degree $n$, there exists $ c_i \crbr{ 0 \le i \le n - 1 } $ such that
\begin{equation}
f - g = \sume{i}{0}{ n - 1 }{ c_i L_i }.
\end{equation}
Therefore,
\begin{equation}
\begin{split}
\norm{f}^2 &= \norm{ g + \sume{i}{0}{ n - 1 }{ c_i L_i }}^2 \\
&= \norm{g}^2 + \sume{i}{0}{ n - 1 }{ c_i^2 \norm{L_i}^2 }
\end{split}
\end{equation}
where the last equality follows from the orthogonality of $L_i$. Because $ \norm{L_i}^2 > 0 $, we have $ \norm{f} \ge \norm{g} $, and the equality is reached iff $ c_i = 0 \crbr{ 0 \le i \le n - 1 } $, which is equivalent to $ f = g $. Consequently,
\begin{gather}
g = \argmin_{ f \mtx{monic}, \deg f = n } \norm{f}, \\
\norm{g} = \min_{ f \mtx{monic}, \deg f = n } \norm{f}.
\end{gather}

\sqed
\end{thmproof}
\end{thmquestion}

\begin{thmanswer}
\ 
\begin{thmquestion}
Suppose the best uniform approximation is $ g \rbr{x} = a x + b $, and therefore there exists a Chebyshev alternance of $3$ points for the $ R \rbr{x} = \sin \frac{ \spi x }{2} - a x - b $. Becuase $R$ is concave over $ \rbr{ 0, 1 } $, therefore two of the points are $ 0, 1 $ respectively. Because $ R \rbr{0} = R \rbr{1} $, it follows that $ a = 1 $ and consequently the third point is
\begin{equation}
\xi = \frac{2}{\spi} \arccos \frac{2}{\spi}.
\end{equation}
From $ R \rbr{0} = -R \rbr{\xi} $, we derive that
\begin{equation}
b = \frac{1}{2} \sin \arccos \frac{2}{\spi} - \frac{1}{\spi} \arccos \frac{2}{\spi} =  \frac{\sqrt{ \spi^2 - 4 }}{ 2 \spi } - \frac{1}{\spi} \arccos \frac{2}{\spi}
\end{equation}
and
\begin{equation}
g \rbr{x} = x + \frac{\sqrt{ \spi^2 - 4 }}{ 2 \spi } - \frac{1}{\spi} \arccos \frac{2}{\spi}.
\end{equation}
\end{thmquestion}
\end{thmanswer}

\begin{thmanswer}
\ 
\begin{thmquestion}
Let $T_n$ be the Chebyshev polynomial of degree $n$, $ r_n = \frac{1}{2^{ n - 1 }} T_n $ and $ f_n = x^n - r_n $. Because $r_n$ is monic, therefore $ f_n \in \mathcal{P}_{ n - 1 } $.

Note that $ r_n = x^n - f_n $ have a Chebyshev alternance of $ n + 1 $ points: let
\begin{equation}
x_k = \cos \frac{ k \spi }{ 2 n }, \crbr{ 0 \le k \le n },
\end{equation}
and then
\begin{partlist}
\item $x_k$ are $ n + 1 $ distinct points arranged from right to left on the axis;
\item
\begin{equation}
r_n \rbr{x_k} = \frac{1}{2^{ n - 1 }} T_n \rbr{x_k} = \frac{1}{2^{ n - 1 }} \rbr{-1}^k;
\end{equation}
\item $ \abs{ r_n \rbr{x} } \le \frac{1}{2^{ n - 1 }} $; \label{Item:NormBound}
\item the equality in \ref{Item:NormBound} is only reached at $x_k$.
\end{partlist}
Because $ f_n \in \mathcal{P}_{ n - 1 } $, therefore $f_n$ is the best uniform approximation of $x^n$.

In conclusion, $ f_n = x^n - \frac{1}{2^{ n - 1 }} T_n $ is the best uniform approximation of $x^n$, and the Chebyshev alternance consists of $ x_k = \cos \frac{ k \spi }{ 2 n } \crbr{ 0 \le k \le n } $.
\end{thmquestion}
\end{thmanswer}

\begin{thmquestion}
\
\begin{thmproof}
Consider
\begin{equation}
u_i = \msbr{ \phi_i \rbr{x_1} & \phi_i \rbr{x_2} & \phi_i \rbr{x_3} & \cdots & \phi_i \rbr{x_{ i + 1 }} }^{\rmut}
\end{equation}
and the matrix
\begin{equation}
M = \msbr{ u_i & u_1 & u_2 & u_3 & \cdots & u_i }.
\end{equation}
Because $M$ is linear dependent in terms of columns, we have
\begin{align}
0 &= \det M \\
&= \sume{j}{1}{n}{ \rbr{-1}^{ j + 1 } \phi_i \rbr{x_j} \rbr{x_j} D_j } \\
&= -\sume{j}{1}{n}{ \phi_i \rbr{x_j} \sigma_j }.
\end{align}
Therefore,
\begin{equation}
\sume{j}{1}{n}{ \phi_i \rbr{x_j} \sigma_j } = 0
\end{equation}
follows as desired.

\sqed
\end{thmproof}
\end{thmquestion}

\begin{thmquestion}
\ 
\begin{thmanswer}
The Python code is placed in the file \verb"Problem8.ipynb". The algorithm succeeded in converging in the $ k = 2 $nd iteration, such that
\begin{equation}
\maxe{j}{1}{ n + 1 }{\abs{\epsilon^{\rbr{k}}_j}} - \mine{j}{1}{ n + 1 }{\abs{\epsilon^{\rbr{k}}_j}} = \text{8.720947e-06} < \text{1e-4}.
\end{equation}
\end{thmanswer}
Plot of $f$ and $p_{\cdot}$ is shown in Figure \ref{Fig:Origin}, and plot of residue is shown in Figure \ref{Fig:Residue}.
\begin{figure}[htbp]
\centering \scalebox{0.8}{\input{Figure-000.pgf}}
\caption{Graph of $f$ and $p_{\cdot}$} \label{Fig:Origin}
\end{figure}
\begin{figure}[htbp]
\centering \scalebox{0.8}{\input{Figure-001.pgf}}
\caption{Graph of $ p_2 - f $} \label{Fig:Residue}
\end{figure}
The final polynomial is
\begin{equation}
\begin{split}
p_2 \rbr{x} &= - 9.600345 \cdot 10^{-11} x^{5} + 0.603579 x^{4} \\
&+ 1.136689 \cdot 10^{-10} x^{3} + 0.414182 x^{2} - 1.766548 \cdot 10^{-11} x - 0.008881,
\end{split}
\end{equation}
while the final control points are
\begin{equation}
-1.000000, -0.832979, -0.414353, -0.000000, 0.414353, 0.832979, 1.000000.
\end{equation}
\end{thmquestion}

\begin{thmquestion}
\
\begin{thmproof}
Consider the space to be continuos function on an interval $ \sbr{ a, b } $ and the inner product to be
\begin{equation}
\pbr{ f, g } = \intb{a}{b}{ f \rbr{x} g \rbr{x} \sd x }.
\end{equation}

Suppose zeros of $p_i$ are $ \xi_1 < \xi_2 < \cdots < \xi_k $ with $ k < i $, and without loss of generality assume $p_i$ are positive, negative, positive, \ldots on $ \rsbr{ \xi_k, b }, \rbr{ \xi_{ k - 1 }, \xi_k }, \cdots, \rbr{ \xi_1, \xi_2 }, \srbr{ a , \xi_1 } $ respectively. Consider
\begin{equation}
g = \rbr{ x - \xi_1 } \rbr{ x - \xi_2 } \cdots \rbr{ x - \xi_k }.
\end{equation}
Because $ p_i g \ge 0 $, and $ p_i g $ have some strictly positive points, therefore
\begin{equation}
\pbr{ p_i, g } = \intb{a}{b}{ p_i \rbr{x} g \rbr{x} \sd x } > 0.
\end{equation}
However, because $ \deg g = k < i $, therefore $ g \in \opspan \cbr{ p_0, p_1, \cdots, p_{ i - 1 } } $ and $ \pbr{ p_i, g } = 0 $, which leads to contradiction. Consequently, $p_i$ has at least $i$ zeros. Because $p_i$ is a polynomial of degree $i$, $p_i$ has exactly $i$ zeros in $ \sbr{ a, b } $.
\end{thmproof}
\end{thmquestion}

\end{document}
